src/MicroSail/Syntax.v
@@ -412,7 +412,7 @@ Module Terms (typekit : TypeKit) (termkit : TermKit typekit).
   Definition LocalStore (Γ : Ctx (𝑿 * Ty)) : Type := NamedEnv Lit Γ.
   Bind Scope env_scope with LocalStore.
 
-  Section Expressions.
+  Section BinaryOperations.
 
     Inductive BinOp : Ty -> Ty -> Ty -> Set :=
     | binop_plus              : BinOp ty_int ty_int ty_int
@@ -426,6 +426,58 @@ Module Terms (typekit : TypeKit) (termkit : TermKit typekit).
     | binop_or                : BinOp ty_bool ty_bool ty_bool
     | binop_pair {σ1 σ2 : Ty} : BinOp σ1 σ2 (ty_prod σ1 σ2)
     | binop_cons {σ : Ty}     : BinOp σ (ty_list σ) (ty_list σ).
+
+  Definition binop_eqb {σ1 σ2 σ3 τ1 τ2 τ3} (op1 : BinOp σ1 σ2 σ3) (op2 : BinOp τ1 τ2 τ3) : bool :=
+    match op1 , op2 with
+    | binop_plus  , binop_plus   => true
+    | binop_times , binop_times  => true
+    | binop_minus , binop_minus  => true
+    | binop_eq    , binop_eq     => true
+    | binop_le    , binop_le     => true
+    | binop_lt    , binop_lt     => true
+    | binop_gt    , binop_gt     => true
+    | binop_and   , binop_and    => true
+    | binop_or    , binop_or     => true
+    | binop_pair  , binop_pair   => if Ty_eq_dec σ3 τ3 then true else false
+    | binop_cons  , binop_cons   => if Ty_eq_dec σ3 τ3 then true else false
+    | _           , _            => false
+    end.
+
+  Inductive OpEq {σ1 σ2 σ3} (op1 : BinOp σ1 σ2 σ3) : forall τ1 τ2 τ3, BinOp τ1 τ2 τ3 -> Prop :=
+  | opeq_refl : OpEq op1 op1.
+  Derive Signature for OpEq.
+  Global Arguments opeq_refl {_ _ _ _}.
+
+  Lemma binop_eqb_spec {σ1 σ2 σ3 τ1 τ2 τ3} (op1 : BinOp σ1 σ2 σ3) (op2 : BinOp τ1 τ2 τ3) :
+    reflect (OpEq op1 op2) (binop_eqb op1 op2).
+  Proof.
+    destruct op1, op2; cbn;
+      try (destruct Ty_eq_dec);
+      try match goal with
+          | H: ty_prod _ _ = ty_prod _ _ |- _ => inversion H; subst; clear H
+          | H: ty_list _   = ty_list _   |- _ => inversion H; subst; clear H
+          end;
+      first
+        [ constructor; constructor
+        | constructor;
+          let H := fresh in
+          intro H;
+          dependent destruction H;
+          congruence
+        ].
+  Defined.
+
+  Lemma binop_eq_dec {σ1 σ2 σ3 τ1 τ2 τ3} (op1 : BinOp σ1 σ2 σ3) (op2 : BinOp τ1 τ2 τ3) :
+    {OpEq op1 op2} + {~ OpEq op1 op2}.
+  Proof.
+    destruct (binop_eqb_spec op1 op2).
+    - left; auto.
+    - right; auto.
+  Defined.
+
+  End BinaryOperations.
+
+  Section Expressions.
 
     (* Intrinsically well-typed expressions. The context Γ of mutable variables
        contains names 𝑿 and types Ty, but the names are not computationally
